Fixed a bug with the modelling of the SBCS and RSCS instructions. Magnus spotting that the carry-out was not being computed correctly. The specification is now simpler.
(Also, for now, have dropped the UNPREDICATBLE predicate.)

examples/elliptic/arm/arm_evalLib.sml
@@ -67,7 +67,7 @@ val _ = Lib.C add_thms arm_compset
    CPSR_WRITE_n2w,SPSR_WRITE_n2w,mode_reg2num_def,mode2psr_def,
    REG_READ_def,REG_WRITE_def,INC_PC_def,FETCH_PC_def,REG_READ6_def,
    word_modify_PSR,word_modify_PSR2,
-   ALU_arith_def,ALU_arith_neg_def,ALU_logic_def,SUB_def,ADD_def,
+   ALU_arith_def,ALU_logic_def,SUB_def,ADD_def,
    AND_def,EOR_def,ORR_def,ALU_def,
    LSL_def,LSR_def,ASR_def,ROR_def,
    WORD_ONLY_RULE `ireg` CONDITION_PASSED_def,CONDITION_PASSED2_def,
